finished the transitivity proof of obs_equiv

src/coq/Effects.v
@@ -10,6 +10,7 @@
 
 Require Import ZArith List String Omega.
 Require Import  Vellvm.Classes Vellvm.Util.
+Require Import Program Classical.
 Require Import paco.
 Import ListNotations.
 
@@ -64,7 +65,7 @@ CoInductive Obs X :=
 | Ret : X -> Obs X        (* Unfinished trace *)
 | Fin : value -> Obs X    (* Finished trace *) 
 | Err : string -> Obs X   (* Abort with an error *)
-| Tau : Obs X -> Obs X      (* Internal step of computation *)
+| Tau : Obs X -> Obs X    (* Internal step of computation *)
 | Eff : effects (Obs X) -> Obs X    (* Externally visible step of computation *)
 .
 
@@ -77,7 +78,12 @@ CoFixpoint obs_map {A B} (f:A -> B) (d:Obs A) : Obs B :=
     | Eff m => Eff (effects_map (obs_map f) m)
   end.
 
-Section UNFOLDING.
+Instance Obs_functor : @Functor Obs := fun A => fun B => @obs_map A B.
+(* A functor only up to stuttering equivalence. *)
+(*
+Program Instance OBS_functor_eq_laws : (@FunctorLaws D) OBS_functor (@obs_equiv).
+*)
+
 
 Definition id_match_obs {A} (d:Obs A) : Obs A :=
   match d with
@@ -93,94 +99,96 @@ Lemma id_obs_eq : forall A (d:Obs A),
 Proof.
   destruct d; auto.
 Qed.
-
-End UNFOLDING.
-
 Arguments id_obs_eq {_} _ .
 
 
-(* Error predicate, which says whether an observation trace leads to an error *)
-Inductive obs_error_free_mem_step {A} (R: Obs A -> Prop) : effects (Obs A) -> Prop :=
-| obs_error_free_mem_Alloca : forall t f, (forall (a:addr), R (f (inj_addr a))) -> obs_error_free_mem_step R (Alloca t f)
-| obs_error_free_mem_Load   : forall a f, (forall (dv:value), R (f dv)) -> obs_error_free_mem_step R (Load a f)
-| obs_error_free_mem_Store  : forall a n d, R d -> obs_error_free_mem_step R (Store a n d)
-| obs_error_free_mem_Call   : forall v vs f, (forall (dv:value), R (f dv)) -> obs_error_free_mem_step R (Call v vs f)
-.                                                                                
+Definition non_tau {A} (d:Obs A) : Prop :=
+  match d with
+  | Tau _ => False
+  | _ => True
+  end.
 
-(* No cases for Ret or Err --
-   Ret means an "unfinished" computation (and shouldn't arise in the semantics of a CFG program)
-   Err definitely has an error, which this predicate rules out
-*)
-Inductive obs_error_free_step {A} (R:Obs A -> Prop) : Obs A -> Prop :=
-| obs_error_free_step_fin : forall v, obs_error_free_step R (Fin v)
-| obs_error_free_step_tau : forall d, R d -> obs_error_free_step R (Tau d)
-| obs_error_free_step_eff : forall m, obs_error_free_mem_step R m -> obs_error_free_step R (Eff m)
-.                                                                             
-Hint Constructors obs_error_free_mem_step obs_error_free_step.
+Definition tau {A} (d:Obs A) : Prop :=
+  match d with
+  | Tau _ => True
+  | _ => False
+  end.
 
-Definition obs_error_free {A} := paco1 (@obs_error_free_step A) bot1.
-Hint Unfold obs_error_free.
+(* Define a predicate that holds only of infinite Tau observations a.k.a. silent divergence *)
+Inductive diverges_step {A} (div : Obs A -> Prop) : Obs A -> Prop :=
+| div_tau : forall d, div d -> diverges_step div (Tau d)
+.
+Hint Constructors diverges_step.
 
-Lemma obs_error_free_gen_mon {A} : monotone1 (@obs_error_free_step A).
+Lemma diverges_step_mono : forall {A}, monotone1 (@diverges_step A).
 Proof.
-  unfold monotone1. intros.
-  induction IN; eauto.
-  eapply obs_error_free_step_eff.
-  induction H; constructor; auto.
+  intros A. pmonauto.
 Qed.
-Hint Resolve obs_error_free_gen_mon : paco.
+Hint Resolve diverges_step_mono : paco.
 
-(*
-  This relation doesn't allow any variation in the relations for the memory model.  A more parametric version would:
-    - have an address relation  A : addr -> addr -> Prop  
-    - have a value relation  V : value -> value -> Prop
-*)
-Inductive obs_equiv_mem_step {A} (R:Obs A -> Obs A -> Prop) : effects (Obs A) -> effects (Obs A) -> Prop :=
-| obs_equiv_mem_Alloca : forall t f g, (forall (a:addr), R (f (inj_addr a)) (g (inj_addr a))) -> obs_equiv_mem_step R (Alloca t f) (Alloca t g)
-| obs_equiv_mem_Load  : forall a f g, (forall (dv:value), R (f dv) (g dv)) -> obs_equiv_mem_step R (Load a f) (Load a g)
-| obs_equiv_mem_Store : forall a n d1 d2, (R d1 d2) -> obs_equiv_mem_step R (Store a n d1) (Store a n d2)
-| obs_equiv_mem_Call  : forall v vs f g, (forall (dv:value), R (f dv) (g dv)) -> obs_equiv_mem_step R (Call v vs f) (Call v vs g)
-.    
+Definition diverges {A} := paco1 (@diverges_step A) bot1.
+Hint Unfold diverges.
 
-Inductive obs_equiv_step {A} (R:Obs A -> Obs A -> Prop) : Obs A -> Obs A -> Prop :=
-| obs_equiv_step_ret : forall a, obs_equiv_step R (Ret a) (Ret a)
-| obs_equiv_step_fin : forall v, obs_equiv_step R (Fin v) (Fin v)
-| obs_equiv_step_err : forall s1 s2, obs_equiv_step R (Err s1) (Err s2)
-| obs_equiv_step_tau : forall d1 d2 (equiv:R d1 d2), obs_equiv_step R (Tau d1) (Tau d2)
-| obs_equiv_step_lft : forall d1 d2, obs_equiv_step R d1 d2 -> obs_equiv_step R (Tau d1) d2
-| obs_equiv_step_rgt : forall d1 d2, obs_equiv_step R d1 d2 -> obs_equiv_step R d1 (Tau d2)
-| obs_equiv_step_eff : forall m1 m2, obs_equiv_mem_step R m1 m2 -> obs_equiv_step R (Eff m1) (Eff m2)
-.    
+(* observational equivalence ------------------------------------------------ *)
+Section OBSERVATIONAL_EQUIVALENCE. 
+
+  (*
+  This relation doesn't allow any variation in the relations for the memory model.  
+  A more parametric version would:
+    - a state relation RA : A -> A -> Prop
+    - have an address relation  RAddr : addr -> addr -> Prop  
+    - have a value relation  RValue : value -> value -> Prop
+
+  It builds in the "total" relation for error string observations:
+     Err s1 ~~ Err s2   for any s1, s2     
+     ( Could pass in E : string -> string -> Prop )
+  *)
+
+
+  Variable A : Type.
+  Variable R : Obs A -> Obs A -> Prop.
+
+  Inductive obs_equiv_mem_step  : effects (Obs A) -> effects (Obs A) -> Prop :=
+  | obs_equiv_mem_Alloca : forall t f g, (forall (a:addr), R (f (inj_addr a)) (g (inj_addr a))) -> obs_equiv_mem_step (Alloca t f) (Alloca t g)
+  | obs_equiv_mem_Load   : forall a f g, (forall (dv:value), R (f dv) (g dv)) -> obs_equiv_mem_step (Load a f) (Load a g)
+  | obs_equiv_mem_Store  : forall a n d1 d2, (R d1 d2) -> obs_equiv_mem_step (Store a n d1) (Store a n d2)
+  | obs_equiv_mem_Call   : forall v vs f g, (forall (dv:value), R (f dv) (g dv)) -> obs_equiv_mem_step (Call v vs f) (Call v vs g)
+  .    
+
+  Inductive obs_equiv_step : Obs A -> Obs A -> Prop :=
+  | obs_equiv_step_ret : forall a, obs_equiv_step (Ret a) (Ret a)
+  | obs_equiv_step_fin : forall v, obs_equiv_step (Fin v) (Fin v)
+  | obs_equiv_step_err : forall s1 s2, obs_equiv_step (Err s1) (Err s2)
+  | obs_equiv_step_tau : forall d1 d2 (equiv:R d1 d2), obs_equiv_step (Tau d1) (Tau d2)
+  | obs_equiv_step_lft : forall d1 d2, obs_equiv_step d1 d2 -> obs_equiv_step (Tau d1) d2
+  | obs_equiv_step_rgt : forall d1 d2, obs_equiv_step d1 d2 -> obs_equiv_step d1 (Tau d2)
+  | obs_equiv_step_eff : forall m1 m2, obs_equiv_mem_step m1 m2 -> obs_equiv_step (Eff m1) (Eff m2)
+  .
+End OBSERVATIONAL_EQUIVALENCE.
 
 Hint Constructors obs_equiv_mem_step obs_equiv_step.  (* obs_equiv *)
 
-Lemma obs_equiv_gen_mon A : monotone2 (@obs_equiv_step A).
+Lemma obs_equiv_mem_step_monotone A : forall (R1 R2:Obs A -> Obs A -> Prop)
+                                        (HR: forall d1 d2, R1 d1 d2 -> R2 d1 d2) m1 m2
+                                        (HM:obs_equiv_mem_step R1 m1 m2),
+    obs_equiv_mem_step R2 m1 m2.
+Proof.
+  intros R1 R2 HR m1 m2 HM.
+  dependent destruction HM; constructor; eauto.
+Qed.  
+Hint Resolve obs_equiv_mem_step_monotone : paco.  
+                                        
+
+Lemma obs_equiv_step_monotone A : monotone2 (@obs_equiv_step A).
 Proof.
   unfold monotone2. intros. induction IN; eauto.
-  eapply obs_equiv_step_eff. induction H.
-  - constructor. eauto.
-  - constructor. eauto.
-  - constructor. eauto.
-  - constructor. eauto.
+  eapply obs_equiv_step_eff. eapply obs_equiv_mem_step_monotone. exact LE. exact H.
 Qed.
-Hint Resolve obs_equiv_gen_mon : paco.
+Hint Resolve obs_equiv_step_monotone : paco.
 
 Definition obs_equiv {A} (p q: Obs A) := paco2 (@obs_equiv_step A) bot2 p q.
 Hint Unfold obs_equiv.
 
-Fixpoint taus {A} (n:nat) (d:Obs A) : Obs A :=
-  match n with
-  | 0 => d
-  | S n => Tau (taus n d)
-  end.
-
-Instance Obs_functor : @Functor Obs := fun A => fun B => @obs_map A B.
-
-
-(* A functor only up to stuttering equivalence. *)
-(*
-Program Instance OBS_functor_eq_laws : (@FunctorLaws D) OBS_functor (@obs_equiv).
-*)
 Lemma obs_equiv_refl : forall {A}, reflexive (Obs A) obs_equiv.
 Proof.
   intro A. pcofix CIH. intro d.
@@ -192,12 +200,11 @@ Lemma obs_equiv_symm : forall {A}, symmetric (Obs A) obs_equiv.
 Proof.
   intro. pcofix CIH.
   intros d1 d2 H.
-  punfold H. remember (upaco2 obs_equiv_step bot2).
+  punfold H. 
   induction H; eauto; subst.
-  - pfold. constructor. right. eapply CIH.
-    destruct equiv; eauto. inversion H. 
-  - pfold. constructor. punfold IHobs_equiv_step.
-  - pfold. constructor. punfold IHobs_equiv_step.
+  - pfold. constructor. right. pclearbot.  eauto. 
+  - pfold. constructor; auto. punfold IHobs_equiv_step.
+  - pfold. constructor; auto. punfold IHobs_equiv_step.
   - pfold. constructor. inversion H; subst.
     + constructor. intro. specialize (H0 a). destruct H0.
       right. eapply CIH. eapply H0. inversion H0.
@@ -208,122 +215,307 @@ Proof.
       right. eapply CIH. eapply H0. inversion H0.
 Qed.
 
+Lemma tau_head_dec : forall {A} (d:Obs A), (exists d', d = Tau d') \/ non_tau d.
+Proof.
+  intros.
+  destruct d; try solve [right; simpl; auto].
+  left. exists d. reflexivity.
+Qed.  
+
+
+Inductive tau_star {A} (P:Obs A -> Prop) : Obs A  -> Prop :=
+| tau_star_zero : forall (d:Obs A), P d -> tau_star P d
+| tau_star_tau  : forall (d:Obs A), tau_star P d -> tau_star P (Tau d)
+.                                                       
+Hint Constructors tau_star.
+
+Lemma tau_star_monotone : forall {A}, monotone1 (@tau_star A).
+Proof.
+  intros A. unfold monotone1.
+  intros x0 r r' IN LE.
+  induction IN; auto.
+Qed.  
+Hint Resolve tau_star_monotone : paco.
+
+(* This prediate relates two traces that agree on a non-tau step *)
+Inductive obs_sync {A} (R: Obs A -> Obs A -> Prop) : Obs A -> Obs A -> Prop :=
+| obs_sync_ret : forall a, obs_sync R (Ret a) (Ret a)
+| obs_sync_fin : forall v, obs_sync R (Fin v) (Fin v)
+| obs_sync_err : forall s1 s2, obs_sync R (Err s1) (Err s2)
+| obs_sync_eff : forall m1 m2, obs_equiv_mem_step R m1 m2 -> obs_sync R (Eff m1) (Eff m2)
+.
+Hint Constructors obs_sync.
+
+Lemma obs_sync_monotone : forall {A}, monotone2 (@obs_sync A).
+Proof.
+  intros A. unfold monotone2.
+  intros x0 x1 r r' IN LE.
+  induction IN; auto.
+  induction H; constructor; auto.
+Qed.
+
+Inductive obs_equiv_big_step {A} (R:Obs A -> Obs A -> Prop) : Obs A -> Obs A -> Prop :=
+| obs_equiv_big_diverge s1 s2 (DS1:diverges s1) (DS2:diverges s2) : obs_equiv_big_step R s1 s2
+| obs_equiv_big_taus s1 s2 t1 t2
+                     (TS1:tau_star (fun t => t = t1) s1)
+                     (TS2:tau_star (fun t => t = t2) s2)
+                     (HO: obs_sync R t1 t2) : obs_equiv_big_step R s1 s2
+.                                                                 
+Hint Constructors obs_equiv_big_step.
+
+Lemma obs_equiv_big_step_monotone : forall {A}, monotone2 (@obs_equiv_big_step A).
+Proof.
+  intros A. unfold monotone2.
+  intros x0 x1 r r' IN LE.
+  induction IN; auto.
+  eapply obs_equiv_big_taus. apply TS1. apply TS2.
+  eapply obs_sync_monotone. apply HO. exact LE.
+Qed.  
+Hint Resolve obs_equiv_big_step_monotone : paco.
+
+Definition obs_equiv_big {A} (d1 d2:Obs A) := paco2 obs_equiv_big_step bot2 d1 d2.
+Hint Unfold obs_equiv_big.
+
+Lemma obs_equiv_tau_lft : forall {A} (d1 d2:Obs A), obs_equiv d1 d2 -> obs_equiv (Tau d1) d2.
+Proof.
+  intros.
+  pfold. apply obs_equiv_step_lft.
+  punfold H.
+Qed.  
+
+Lemma obs_equiv_tau_rgt : forall {A} (d1 d2:Obs A), obs_equiv d1 d2 -> obs_equiv d1 (Tau d2).
+Proof.
+  intros.
+  pfold. apply obs_equiv_step_rgt.
+  punfold H.
+Qed.  
 
 Lemma obs_equiv_lft_inversion : forall {A} (d1 d2:Obs A), obs_equiv (Tau d1) d2 -> obs_equiv d1 d2.
 Proof.
-  intros A d1 d2 H.  punfold H. remember (Tau d1) as d. induction H; try (inversion Heqd; subst; clear Heqd).
-  - pfold. constructor. pclearbot. 
-    destruct equiv. eapply obs_equiv_gen_mon.
-    eapply SIM. eapply LE.
-  - pfold. eapply H.
-  - pfold. constructor.
-    apply IHobs_equiv_step in Heqd.
-    punfold Heqd.
-Qed. 
+  intros A. intros d1 d2 H.
+  punfold H. remember (Tau d1) as d. 
+  induction H; try (solve [inversion Heqd; subst; clear Heqd]).
+  - inversion Heqd. subst. apply obs_equiv_tau_rgt. pclearbot. punfold equiv.
+  - inversion Heqd. subst. pfold. exact H.
+  - subst. apply obs_equiv_tau_rgt. apply IHobs_equiv_step. reflexivity.
+Qed.    
 
-Lemma stutter_simpl : forall {A} (d1 d2: Obs A) n, obs_equiv (taus n d1) d2 -> obs_equiv d1 d2.
-Proof.
-  intros. induction n. punfold H.
-  eapply IHn. simpl in H. eapply obs_equiv_lft_inversion. eapply H.
-Qed.
-
-Lemma stutter : forall {A} (d1 d2: Obs A) n m, obs_equiv (taus n d1) (taus m d2) -> obs_equiv d1 d2.
+Lemma obs_equiv_rgt_inversion : forall {A} (d1 d2:Obs A), obs_equiv d1 (Tau d2) -> obs_equiv d1 d2.
 Proof.
   intros.
-  eapply stutter_simpl.
-  eapply obs_equiv_symm.
-  eapply stutter_simpl.
-  eapply obs_equiv_symm.
-  eauto.
+  apply obs_equiv_symm. apply obs_equiv_symm in H. apply obs_equiv_lft_inversion. exact H.
+Qed.  
+
+Lemma sync_not_diverges : forall {A} (d:Obs A), tau_star non_tau d -> diverges d -> False.
+Proof.
+  intros A d HS.
+  induction HS.
+  - intros HD; dependent destruction d; punfold HD; inversion HD.
+  - intros HD. apply IHHS. punfold HD. dependent destruction HD. pclearbot. apply H.
+Qed.    
+
+(* CLASSICAL! *)
+Lemma sync_or_diverges : forall {A} (d:Obs A), tau_star non_tau d \/ diverges d.
+Proof.
+  intros A d.
+  destruct (classic (tau_star non_tau d)); eauto.
+  right. revert d H.
+  pcofix CIH.
+  intros d H.
+  destruct d; try solve [exfalso; apply H; constructor; simpl; auto].
+  pfold. econstructor. right. eauto.
 Qed.
 
-
-Lemma obs_equiv_step_transitive:  forall A R, transitive (Obs A) R -> transitive (Obs A) (obs_equiv_step R).
+Lemma obs_equiv_diverges : forall {A} (d1 d2:Obs A) (EQ: obs_equiv d1 d2) (HD:diverges d1), diverges d2.
 Proof.
   intros A.
-  unfold relation. unfold transitive.
-  intros R Ht.
-  intros x y z H. generalize dependent z.
-  induction H; intros z H1. 
-  - remember (Ret a) as w. induction H1; inversion Heqw; eauto.
-    subst. apply obs_equiv_step_rgt. exact H1.
-  - remember (Fin v) as w. induction H1; inversion Heqw; eauto.
-    subst. apply obs_equiv_step_rgt. exact H1.
-  - remember (Err s2) as w. induction H1; inversion Heqw; eauto.
-  - apply obs_equiv_step_lft. generalize dependent d1. remember (Tau d2) as w.
-    induction H1; inversion Heqw; subst; intros d1 HR.
-    apply obs_equiv_step_rgt. 
-Abort.    
-  
+  pcofix CIH.
+  intros d1 d2 EQ.
+  punfold EQ. induction EQ; intros HD; try solve [punfold HD; inversion HD].
+  - punfold HD. inversion HD. pclearbot. subst.
+    pfold. constructor. right. eauto.
+  - punfold HD. inversion HD. subst. pclearbot. apply IHEQ. apply H0.
+  - pfold. constructor. left. auto.
+Qed.    
 
+Lemma obs_equiv_sync : forall {A} (d1 d2:Obs A) (EQ:obs_equiv d1 d2) (HS:tau_star non_tau d1), tau_star non_tau d2.
+Proof.
+  intros A d1 d2 EQ HS.
+  revert d2 EQ.
+  induction HS; intros d2 EQ.
+  - punfold EQ. induction EQ; auto.
+    inversion H.
+  - punfold EQ. dependent induction EQ.
+    + apply tau_star_tau. apply IHHS. pclearbot. eauto.
+    + apply IHHS. pfold. exact EQ.
+    + apply tau_star_tau. eauto.
+Qed.      
+
+Lemma obs_equiv_diverges_or_sync : forall {A} (d1 d2:Obs A) (EQ:obs_equiv d1 d2),
+    (diverges d1 /\ diverges d2) \/ (tau_star non_tau d1 /\ tau_star non_tau d2).
+Proof.
+  intros A d1 d2 EQ.
+  destruct (@sync_or_diverges _ d1) as [HS | HD].
+  - right. eauto using obs_equiv_sync.
+  - left. eauto using obs_equiv_diverges.
+Qed.    
+
+Lemma obs_equiv_big_step_tau_left :  forall {A} R (d1 d2:Obs A)
+                                       (HR: paco2 obs_equiv_big_step R d1 d2), paco2 obs_equiv_big_step R (Tau d1) d2.
+Proof.
+  intros A R d1 d2 HR.
+  punfold HR.
+  pfold.
+  destruct HR.
+  - apply obs_equiv_big_diverge; eauto. pfold. constructor. left. eauto.
+  - eapply obs_equiv_big_taus; eauto.
+Qed.
+
+Lemma obs_equiv_big_step_tau_right :  forall {A} R (d1 d2:Obs A)
+                                       (HR: paco2 obs_equiv_big_step R d1 d2), paco2 obs_equiv_big_step R d1 (Tau d2).
+Proof.
+  intros A R d1 d2 HR.
+  punfold HR.
+  pfold.
+  destruct HR.
+  - apply obs_equiv_big_diverge; eauto. pfold. constructor. left. eauto.
+  - eapply obs_equiv_big_taus; eauto.
+Qed.
+
+Lemma obs_equiv_implies_obs_equiv_big: forall {A} (d1 d2:Obs A) (EQ:obs_equiv d1 d2), obs_equiv_big d1 d2.
+Proof.
+  intros A.
+  pcofix CIH.
+  intros d1 d2 EQ.
+  destruct (@obs_equiv_diverges_or_sync _ d1 d2 EQ) as [[HD1 HD2]|[HS1 HS2]]; eauto.
+  induction HS1.
+  - induction HS2.
+    + pfold. eapply obs_equiv_big_taus; try solve [eauto].
+      punfold EQ. dependent destruction EQ; eauto; try solve [simpl in H; inversion H]; try solve [simpl in H0; inversion H0].
+      constructor.
+      apply obs_equiv_mem_step_monotone with (R1 := (upaco2 (obs_equiv_step (A:=A)) bot2)).
+      intros d1 d2 H2. right.  eapply CIH. pclearbot. eapply H2.
+      exact H.
+    + eauto using obs_equiv_big_step_tau_right, obs_equiv_rgt_inversion.
+  - eauto using obs_equiv_big_step_tau_left, obs_equiv_lft_inversion.
+Qed.
+      
+Lemma obs_equiv_big_implies_obs_equiv : forall {A} (d1 d2:Obs A) (EQB:obs_equiv_big d1 d2), obs_equiv d1 d2.
+Proof.
+  intros A.
+  pcofix CIH.
+  intros d1 d2 EQB.
+  punfold EQB. dependent destruction EQB.
+  - punfold DS1. punfold DS2.
+    dependent destruction DS1. dependent destruction DS2.
+    pfold. econstructor; eauto. right. apply CIH. pclearbot.
+    pfold. eapply obs_equiv_big_diverge; eauto.
+  - dependent induction TS1; subst.
+    + dependent induction TS2; subst.
+      * pfold. dependent destruction HO; eauto.
+        constructor. eapply obs_equiv_mem_step_monotone with (R1 := (upaco2 obs_equiv_big_step bot2)).
+        intros. right. apply CIH. pclearbot. eauto.
+        exact H.
+      * pfold.  apply IHTS2 in HO. punfold HO.
+    + pfold. constructor. apply IHTS1 in TS2; eauto. punfold TS2.
+Qed.      
+
+Lemma obs_sync_non_tau_left : forall {A} R (d1 d2:Obs A), obs_sync R d1 d2 -> non_tau d1.
+Proof.
+  intros A R d1 d2 H.
+  dependent destruction H; simpl; auto.
+Qed.
+
+Lemma obs_sync_non_tau_right : forall {A} R (d1 d2:Obs A), obs_sync R d1 d2 -> non_tau d2.
+Proof.
+  intros A R d1 d2 H.
+  dependent destruction H; simpl; auto.
+Qed.
+
+Lemma tau_star_non_tau_unique : forall {A} (d d1 d2:Obs A)
+   (TS1:tau_star (fun s => s = d1) d)
+   (TS2:tau_star (fun s => s = d2) d)
+   (NT1:non_tau d1)
+   (NT2:non_tau d2),
+    d1 = d2.
+Proof.
+  intros A d d1 d2 TS1.
+  revert d2.
+  induction TS1; intros d2 TS2 ND1 ND2.
+  - induction TS2; subst; eauto.
+    + simpl in ND1. inversion ND1.
+  - dependent destruction TS2; eauto.
+    simpl in ND2. inversion ND2.
+Qed.    
+
+Lemma obs_equiv_mem_step_trans:
+  forall {A} (R : relation (Obs A)) (TR:transitive _ R) m1 m2 m3,
+    obs_equiv_mem_step R m1 m2 -> obs_equiv_mem_step R m2 m3 ->
+    obs_equiv_mem_step R m1 m3.
+Proof.
+  intros A R TR m1 m2 m3 H12 H23.
+  inversion H12; subst; inversion H23; subst; constructor; intros; eauto.
+Qed.
+
+Lemma obs_equiv_big_trans : forall {A} (d1 d2 d3:Obs A), obs_equiv_big d1 d2 -> obs_equiv_big d2 d3 -> obs_equiv_big d1 d3.
+Proof.
+  intros A.
+  pcofix CIH.
+  intros d1 d2 d3 EQB1 EQB2.
+  punfold EQB1. punfold EQB2.
+  destruct EQB1, EQB2; eauto.
+  - exfalso. eapply sync_not_diverges, DS2.
+    eapply tau_star_monotone. apply TS1.
+    intros s PR. simpl in PR.  subst. eauto using obs_sync_non_tau_left.
+  - exfalso. eapply sync_not_diverges, DS1.
+    eapply tau_star_monotone. apply TS2.
+    intros s PR. simpl in PR. subst. eauto using obs_sync_non_tau_right.
+  - eapply tau_star_non_tau_unique in TS2; eauto using obs_sync_non_tau_left, obs_sync_non_tau_right.
+    subst.
+    pfold. eapply obs_equiv_big_taus; eauto.
+    destruct HO; dependent destruction HO0; eauto.
+    econstructor.
+
+    dependent destruction H; dependent destruction H0.
+    + constructor.  
+      intros a. specialize H0 with (a:=a).  specialize H with (a:=a). pclearbot.
+      right. eapply CIH; eauto.
+    + constructor.  
+      intros dv. specialize H0 with (dv:=dv).  specialize H with (dv:=dv). pclearbot.
+      right. eapply CIH; eauto.
+    + constructor.
+      right. pclearbot. eauto.
+    + constructor.
+      intros dv. specialize H0 with (dv := dv). specialize H with (dv:=dv). pclearbot.
+      right. eauto.
+Qed.    
+    
 
 Lemma obs_equiv_trans : forall {A} (d1 d2 d3: Obs A), obs_equiv d1 d2 -> obs_equiv d2 d3 -> obs_equiv d1 d3.
 Proof.
-  intro A. pcofix CIH.
-  intros d1 d2 d3 H1 H2.
-  pfold.
-  punfold H1. remember (upaco2 obs_equiv_step bot2) as R.
-  generalize dependent d3.
-  induction H1; intros d3 H2.
-  - punfold H2. rewrite <- HeqR in H2. remember (Ret a) as d2.
-    induction H2; try inversion Heqd2; eauto.
-    apply obs_equiv_step_rgt. subst. apply IHobs_equiv_step in H.  exact H.
-  - punfold H2. rewrite <- HeqR in H2. remember (Fin v) as d2.
-    induction H2; try inversion Heqd2; eauto.
-    apply obs_equiv_step_rgt. subst. apply IHobs_equiv_step in H. exact H.
-  - punfold H2. rewrite <- HeqR in H2. remember (Err s2) as d2.
-    induction H2; try inversion Heqd2; eauto.
-  - punfold H2.
-    rewrite <- HeqR in H2. remember (Tau d2) as d.
-    induction H2; try inversion Heqd; subst; eauto.
-    + pclearbot. destruct equiv. destruct equiv0.
-    apply obs_equiv_step_tau. right. eapply CIH. pfold.
-    eapply obs_equiv_gen_mon. apply SIM. eapply LE.
-    pfold. eapply obs_equiv_gen_mon. eapply SIM0. eapply LE0.
-    + pclearbot. destruct equiv. 
-      apply obs_equiv_step_lft.  eapply obs_equiv_gen_mon.
-Abort.
-      
+  eauto using obs_equiv_big_trans, obs_equiv_implies_obs_equiv_big, obs_equiv_big_implies_obs_equiv.
+Qed.
 
-(* Note: for guardedness, bind Ret introduces extra Tau *)
-Definition bind {A B} (m:Obs A) (f:A -> Obs B) : Obs B :=
-  (cofix bindf := fun m => 
-     match m with
-       | Ret a => Tau (f a)
-       | Fin d => Fin d
-       | Err s => Err s
-       | Tau d' => Tau (bindf d')
-       | Eff m => Eff (effects_map bindf m)
-     end) m.
 
-Lemma binobs_unfold : forall {A B} (m:Obs A) (f:A -> Obs B),
-    obs_equiv (bind m f)
-    (match m with
-    | Ret a => Tau (f a)
-    | Fin d => Fin d
-    | Err s => Err s
-    | Tau d' => Tau (bind d' f)
-    | Eff e => Eff (effects_map (fun m => bind m f) e)
-    end).
+Lemma obs_equiv_step_any_error_r : forall {A} r (d:Obs A) s1 s2,
+    obs_equiv_step r d (Err s1) -> obs_equiv_step r d (Err s2).
 Proof.
-  intros A B.
-  pcofix CIH. intros m f.
-  unfold bind.
-  pfold. destruct m.
-Abort.
-  
-Program Instance Obs_monad : (@Monad Obs) (@Obs_functor) := _.
-Next Obligation.
-  split.
-  - intros. apply Ret. exact X.
-  - intros A B. apply bind.
-Defined.
+  intros A r d s1 s2 H.
+  remember (Err s1) as d1.
+  induction H; try solve [inversion Heqd1].
+  - constructor.
+  - subst. constructor. apply IHobs_equiv_step; auto.
+Qed.    
 
-
-Ltac punfold' H := let x := fresh "_x_" in
-  repeat red in H;
-  let G := type of H in paco_class G (@pacounfold);
-  intro x; match goal with [x:=?lem|-_] => clear x; eapply lem in H end.
+Lemma obs_equiv_step_any_error_l : forall {A} r (d:Obs A) s1 s2,
+    obs_equiv_step r (Err s1) d -> obs_equiv_step r (Err s2) d.
+Proof.
+  intros A r d s1 s2 H.
+  remember (Err s1) as d1.
+  induction H; try solve [inversion Heqd1].
+  - constructor.
+  - subst. constructor. apply IHobs_equiv_step; auto.
+Qed.    
 
 
 Section OBS_EQUIV_COIND.
@@ -361,5 +553,139 @@ End OBS_EQUIV_COIND.
 Arguments obs_equiv_coind [_] _ [_ _] _ _.
 
 
+(* This statement is false if d1 and d2 are inifinite Tau streams
+    would have to weaken the conclusion to:
+      (d1 = d2 /\ d1 = all_taus) \/ ... 
+    this would probably require classical logic to prove.
+
+Lemma obs_equiv_inversion : forall {A} (d1 d2:Obs A),
+    obs_equiv d1 d2 ->  exists d1', exists d2', exists n, exists m,
+            d1 = taus n d1' /\ d2 = taus m d2' /\ non_tau_head d1' /\ non_tau_head d2' /\ obs_equiv d1' d2'.
+Proof.
+Abort.  
+*)
+
+
+(* stuttering --------------------------------------------------------------- *)
+
+Fixpoint taus {A} (n:nat) (d:Obs A) : Obs A :=
+  match n with
+  | 0 => d
+  | S n => Tau (taus n d)
+  end.
+
+Lemma stutter_simpl : forall {A} (d1 d2: Obs A) n, obs_equiv (taus n d1) d2 -> obs_equiv d1 d2.
+Proof.
+  intros. induction n. punfold H.
+  eapply IHn. simpl in H. eapply obs_equiv_lft_inversion. eapply H.
+Qed.
+
+Lemma stutter : forall {A} (d1 d2: Obs A) n m, obs_equiv (taus n d1) (taus m d2) -> obs_equiv d1 d2.
+Proof.
+  intros.
+  eapply stutter_simpl.
+  eapply obs_equiv_symm.
+  eapply stutter_simpl.
+  eapply obs_equiv_symm.
+  eauto.
+Qed.
+
+(* error-free observations -------------------------------------------------- *)
+
+(* Error predicate, which says whether an observation trace leads to an error *)
+Inductive obs_error_free_mem_step {A} (R: Obs A -> Prop) : effects (Obs A) -> Prop :=
+| obs_error_free_mem_Alloca : forall t f, (forall (a:addr), R (f (inj_addr a))) -> obs_error_free_mem_step R (Alloca t f)
+| obs_error_free_mem_Load   : forall a f, (forall (dv:value), R (f dv)) -> obs_error_free_mem_step R (Load a f)
+| obs_error_free_mem_Store  : forall a n d, R d -> obs_error_free_mem_step R (Store a n d)
+| obs_error_free_mem_Call   : forall v vs f, (forall (dv:value), R (f dv)) -> obs_error_free_mem_step R (Call v vs f)
+.                                                                                
+
+(* No cases for Ret or Err --
+   Ret means an "unfinished" computation (and shouldn't arise in the semantics of a CFG program)
+   Err definitely has an error, which this predicate rules out
+*)
+Inductive obs_error_free_step {A} (R:Obs A -> Prop) : Obs A -> Prop :=
+| obs_error_free_step_fin : forall v, obs_error_free_step R (Fin v)
+| obs_error_free_step_tau : forall d, R d -> obs_error_free_step R (Tau d)
+| obs_error_free_step_eff : forall m, obs_error_free_mem_step R m -> obs_error_free_step R (Eff m)
+.                                                                             
+Hint Constructors obs_error_free_mem_step obs_error_free_step.
+
+Definition obs_error_free {A} := paco1 (@obs_error_free_step A) bot1.
+Hint Unfold obs_error_free.
+
+Lemma obs_error_free_gen_mon {A} : monotone1 (@obs_error_free_step A).
+Proof.
+  unfold monotone1. intros.
+  induction IN; eauto.
+  eapply obs_error_free_step_eff.
+  induction H; constructor; auto.
+Qed.
+Hint Resolve obs_error_free_gen_mon : paco.
+
+
+(* Note: for guardedness, bind Ret introduces extra Tau *)
+(*
+Definition bind {A B} (m:Obs A) (f:A -> Obs B) : Obs B :=
+  (cofix bindf := fun m => 
+     match m with
+       | Ret a => Tau (f a)
+       | Fin d => Fin d
+       | Err s => Err s
+       | Tau d' => Tau (bindf d')
+       | Eff m => Eff (effects_map bindf m)
+     end) m.
+*)
+
+CoFixpoint bind {A B} (m:Obs A) (f:A -> Obs B) : Obs B :=
+  match m with
+  | Ret a => Tau (f a)
+  | Fin d => Fin d
+  | Err s => Err s
+  | Tau d' => Tau (bind d' f)
+  | Eff e => Eff (effects_map (fun x => bind x f) e)
+  end.
+
+Lemma bind_id_eq : forall {A B} (m:Obs A) (f:A -> Obs B),
+  bind m f =
+  match (bind m f) with
+  | Ret a => Ret a
+  | Fin d => Fin d
+  | Err s => Err s
+  | Tau d' => Tau d'
+  | Eff e => Eff e
+  end.
+Proof.
+  intros.
+  destruct (bind m f); auto.
+Qed.  
+
+Lemma binobs_unfold : forall {A B} (m:Obs A) (f:A -> Obs B),
+    obs_equiv (bind m f)
+    (match m with
+    | Ret a => Tau (f a)
+    | Fin d => Fin d
+    | Err s => Err s
+    | Tau d' => Tau (bind d' f)
+    | Eff e => Eff (effects_map (fun m => bind m f) e)
+    end).
+Proof.
+  intros A B m f. 
+  destruct m; rewrite bind_id_eq; simpl; try eapply obs_equiv_refl.
+Qed.
+  
+  
+Program Instance Obs_monad : (@Monad Obs) (@Obs_functor) := _.
+Next Obligation.
+  split.
+  - intros. apply Ret. exact X.
+  - intros A B. apply bind.
+Defined.
+
+
+Ltac punfold' H := let x := fresh "_x_" in
+  repeat red in H;
+  let G := type of H in paco_class G (@pacounfold);
+  intro x; match goal with [x:=?lem|-_] => clear x; eapply lem in H end.
 
 End Effects.
